graph updating lemmas in hip_graphmark is proved.

hip_graphmark_proofs.v
@@ -6,7 +6,9 @@ Require Import graph_reachable.
 Require Import spatial_graph.
 Require Import hip_graphmark.
 Require Import utilities.
+Require Import ramification.
 Require Import Classical.
+Require Import ramify_tactics.
 Tactic Notation "LEM" constr(v) := (destruct (classic v); auto).
 
 
@@ -35,88 +37,130 @@ Module GraphMark <: Mgraphmark.
   Definition lookup : A -> node -> nat -> node -> node -> formula :=
     fun g x d l r w => @node_label _ _ _ (b_pg_g g) x = d /\ @graph.valid _ _ _ (b_pg_g g) x /\
                        @graph.valid _ _ _ (b_pg_g g) l /\ @graph.valid _ _ _ (b_pg_g g) r /\
-                       (@edge_func _ _ _ (b_pg_g g) x = l :: r :: nil \/ @edge_func _ _ _ (b_pg_g g) x = r :: l :: nil).
+                       @edge_func _ _ _ (b_pg_g g) x = l :: r :: nil.
   Definition update : A -> node -> nat -> node -> node -> A -> formula :=
     fun g1 x d l r g2 w => exists (Hn : x <> 0) (Hi : in_math (bm_ma_g g1) x l r), update_graph g1 x d l r Hi Hn = g2.
 
   Lemma axiom_1 : forall v G1 G2 G G3 x l r, valid (imp (and (lookup G x v l r) (and (mark G r G1) (and (neq v 1) (and (mark G2 l G3) (update G1 x 1 l r G2))))) (and (mark G x G3) (lookup G3 x 1 l r))).
   Proof. admit. Qed.
-  
+
   Lemma axiom_2 : forall v G1 G2 G G3 x l r, valid (imp (and (lookup G x v l r) (and (mark G l G1) (and (neq v 1) (and (mark G2 r G3) (update G1 x 1 l r G2))))) (and (mark G x G3) (lookup G3 x 1 l r))).
   Proof. admit. Qed.
-  
+
   Lemma axiom_3 : forall v G1 G2 G G3 x l r, valid (imp (and (lookup G x v l r) (and (mark G r G1) (and (neq v 1) (and (mark G1 l G2) (update G2 x 1 l r G3))))) (and (mark G x G3) (lookup G3 x 1 l r))).
   Proof. admit. Qed.
-  
+
   Lemma axiom_4 : forall v G1 G2 G G3 x l r, valid (imp (and (lookup G x v l r) (and (mark G l G1) (and (neq v 1) (and (mark G1 r G2) (update G2 x 1 l r G3))))) (and (mark G x G3) (lookup G3 x 1 l r))).
   Proof. admit. Qed.
-  
+
   Lemma axiom_5 : forall v G1 G2 G G3 x l r, valid (imp (and (lookup G x v l r) (and (update G x 1 l r G1) (and (neq v 1) (and (mark G1 r G2) (mark G2 l G3))))) (and (mark G x G3) (lookup G3 x 1 l r))).
   Proof. admit. Qed.
-  
+
   Lemma axiom_6 : forall v G1 G2 G G3 x l r, valid (imp (and (lookup G x v l r) (and (update G x 1 l r G1) (and (neq v 1) (and (mark G1 l G2) (mark G2 r G3))))) (and (mark G x G3) (lookup G3 x 1 l r))).
   Proof.
     intros; intro w; hnf; unfold and; hnf; intros. destruct H as [? [? [? [? ?]]]]. destruct H as [? [? [? [? ?]]]]. hnf in H1.
     assert (mark1 adr nat natEqDec (fun d : nat => d = 1) (b_pg_g G) x (b_pg_g G1)). destruct H0 as [Hi [Hn ?]].
     rewrite <- H0. split. intro z. split. destruct (t_eq_dec z x); split; intro. hnf. left; auto. hnf in H8. subst. auto.
-    left; auto. hnf in H8. destruct H8. auto. exfalso; auto. split; intro t; intros. simpl. unfold change_edge_func.
-    destruct (t_eq_dec z x). destruct H7. subst. rewrite H7 in H8. auto. subst. rewrite H7 in H8. apply in_inv in H8.
-    destruct H8. subst. apply in_cons, in_eq. apply in_inv in H; destruct H. subst. apply in_eq. inversion H. auto. simpl in H8.
-    unfold change_edge_func in H8. destruct (t_eq_dec z x). subst. destruct H7. rewrite H. auto. rewrite H. apply in_inv in H8.
-    destruct H8. subst. apply in_cons, in_eq. apply in_inv in H0; destruct H0. subst. apply in_eq. inversion H0. auto.
-    split. auto. split. hnf. simpl. unfold change_node_label. destruct (@t_eq_dec adr natEqDec x x). auto. exfalso; auto.
-    intros. simpl. unfold change_node_label. destruct (t_eq_dec n' x). exfalso; auto. auto. split.
+    left; auto. hnf in H8. destruct H8. auto. exfalso; auto. simpl. unfold change_edge_func. destruct (t_eq_dec z x).
+    subst. rewrite H7. auto. auto. split. auto. split. hnf. simpl. unfold change_node_label.
+    destruct (@t_eq_dec adr natEqDec x x). auto. exfalso; auto. intros. simpl. unfold change_node_label.
+    destruct (t_eq_dec n' x). exfalso; auto. auto. split.
     apply (mark_mark_mark1 _ _ _ _ (b_pg_g G) (b_pg_g G1) (b_pg_g G2) (b_pg_g G3) x l r). hnf; simpl. rewrite H. auto.
-    split. do 2 (split; auto). destruct H7; rewrite H7. apply in_eq. apply in_cons, in_eq. split. do 2 (split; auto).
-    destruct H7; rewrite H7. apply in_cons, in_eq. apply in_eq. intros. destruct H9 as [?[? ?]].
-    destruct H7; rewrite H7 in H11; apply in_inv in H11; destruct H11. left; auto. apply in_inv in H11. destruct H11.
-    right; auto. inversion H11. right; auto. apply in_inv in H11. destruct H11. left; auto. inversion H11. auto. apply H2.
-    apply H3. destruct H8 as [? [? [? ?]]]. split. hnf in H10. assert (@node_label _ _ _ (b_pg_g G2) x = 1).
-    destruct H2 as [? [? ?]]. specialize (H12 x). specialize (H13 x).
-    LEM ((b_pg_g G1) |= l ~o~> x satisfying (unmarked nat (fun d : nat => d = 1))). specialize (H12 H14). hnf in H12.
-    rewrite H12; auto. specialize (H13 H14). rewrite <- H13. apply H10. destruct H3 as [? [? ?]]. specialize (H13 x).
-    specialize (H14 x). LEM ((b_pg_g G2) |= r ~o~> x satisfying (unmarked nat (fun d : nat => d = 1))). specialize (H13 H15).
-    hnf in H13. auto. specialize (H14 H15). rewrite <- H14. apply H12. destruct H2 as [? _]. destruct H3 as [? _].
+    split. do 2 (split; auto). rewrite H7. apply in_eq. split. do 2 (split; auto). rewrite H7. apply in_cons, in_eq.
+    intros. destruct H9 as [?[? ?]]. rewrite H7 in H11. apply in_inv in H11; destruct H11. left; auto. apply in_inv in H11.
+    destruct H11. right; auto. inversion H11. auto. apply H2. apply H3.
+
+    destruct H8 as [? [? [? ?]]]. split. hnf in H10. assert (@node_label _ _ _ (b_pg_g G2) x = 1). destruct H2 as [? [? ?]].
+    specialize (H12 x). specialize (H13 x). LEM ((b_pg_g G1) |= l ~o~> x satisfying (unmarked nat (fun d : nat => d = 1))).
+    specialize (H12 H14). hnf in H12. rewrite H12; auto. specialize (H13 H14). rewrite <- H13. apply H10.
+    destruct H3 as [? [? ?]]. specialize (H13 x). specialize (H14 x).
+    LEM ((b_pg_g G2) |= r ~o~> x satisfying (unmarked nat (fun d : nat => d = 1))). specialize (H13 H15). hnf in H13. auto.
+    specialize (H14 H15). rewrite <- H14. apply H12. destruct H2 as [? _]. destruct H3 as [? _].
     assert ((b_pg_g G) ~=~ (b_pg_g G2)). apply (si_trans H8 H2). assert ((b_pg_g G) ~=~ (b_pg_g G3)). apply (si_trans H12 H3).
     hnf in H13. split. destruct (H13 x). rewrite <- H14; auto. split. destruct (H13 l). rewrite <- H14; auto. split.
-    destruct (H13 r). rewrite <- H14; auto. specialize (H13 x). destruct H13.
-    destruct H7; rewrite H7 in H14; destruct H14; hnf in H14, H15;
-    destruct (@only_two_neighbours _ _ _ (bm_bi_g G3) x) as [v1 [v2 ?]]; unfold b_pg_g in *; unfold bm_bi_g in *;
-    rewrite e in *; clear e. assert (In l (l :: r :: nil)). apply in_eq. assert (In r (l :: r :: nil)). apply in_cons, in_eq.
-    generalize (H14 l H16); intro. apply in_inv in H18. destruct H18. subst. left. specialize (H14 r H17).
-    destruct (eq_nat_dec v2 r). subst; auto. assert (In v2 (l :: v2 :: nil)) by apply in_cons, in_eq. specialize (H15 v2 H).
-    clear H16 H17. apply in_inv in H14. apply in_inv in H15. destruct H14, H15; exfalso. rewrite H14 in H15. auto.
-    apply in_inv in H15. destruct H15. auto. inversion H15. apply in_inv in H14. destruct H14. auto. inversion H14.
-    apply in_inv in H14. destruct H14. auto. inversion H14. apply in_inv in H18. destruct H18. right. subst.
-    specialize (H14 r H17). destruct (eq_nat_dec v1 r). subst; auto. assert (In v1 (v1 :: l :: nil)) by apply in_eq.
-    specialize (H15 v1 H). clear H16 H17 H. exfalso. apply in_inv in H14. destruct H14. auto. apply in_inv in H.
-    apply in_inv in H15. destruct H, H15. subst. auto. apply in_inv in H14. destruct H14. auto. inversion H14. inversion H.
-    inversion H. inversion H18. assert (In l (r :: l :: nil)). apply in_cons, in_eq. assert (In r (r :: l :: nil)). apply in_eq.
-    generalize (H14 l H16); intro. apply in_inv in H18. destruct H18. subst. left. specialize (H14 r H17).
-    destruct (eq_nat_dec v2 r). subst; auto. assert (In v2 (l :: v2 :: nil)) by apply in_cons, in_eq. specialize (H15 v2 H).
-    clear H16 H17 H. exfalso. apply in_inv in H15. destruct H15. auto. apply in_inv in H. apply in_inv in H14. destruct H, H14.
-    subst. auto. apply in_inv in H14. destruct H14; [auto | inversion H14]. inversion H. inversion H. apply in_inv in H18.
-    destruct H18. subst. right. specialize (H14 r H17). assert (In v1 (v1 :: l :: nil)). apply in_eq. specialize (H15 v1 H).
-    clear H16 H17 H. destruct (eq_nat_dec v1 r). subst; auto. exfalso. apply in_inv in H14. destruct H14. auto.
-    apply in_inv in H15. destruct H15. auto. apply in_inv in H. apply in_inv in H14. destruct H, H14. subst; auto.
-    inversion H14. inversion H. inversion H14. inversion H18.
+    destruct (H13 r). rewrite <- H14; auto. specialize (H13 x). destruct H13. rewrite <- H14. auto.
   Qed.
+
   Lemma axiom_7 : forall v G x G1 y v1 l r, valid (imp (and (mark G x G1) (lookup G y v l r)) (and (subset_reach G x G1) (and (eq_notreach G x G1) (lookup G1 y v1 l r)))).
   Proof. admit. Qed.
-  
+
   Lemma axiom_8 : forall l r x G, valid (imp (lookup G x 1 l r) (mark G x G)).
   Proof. admit. Qed.
-  
+
   Lemma axiom_9 : forall G, valid (mark G null_node G).
   Proof. admit. Qed.
-  
+
+  Lemma lookup_graph_unfold: forall G v x l r w,
+                               lookup G x v l r w -> (graph x G = trinode x v l r ⊗ graph l G ⊗ graph r G)%pred.
+  Proof.
+    intros. destruct H as [? [? [? [? ?]]]]. clear w. apply pred_ext; intro w; intro. rewrite graph_unfold in H4.
+    destruct H4 as [[? ?] | [dd [ll [rr [[? ?] ?]]]]]. hnf in H4. unfold b_pg_g in H0. rewrite <- pg_the_same in H0.
+    apply valid_not_null in H0. exfalso; auto. unfold gamma in H4. unfold biEdge in H4.
+    destruct (@only_two_neighbours adr nat natEqDec (@bm_bi adr nat O natEqDec G) x) as [v1 [v2 ?]] in H4. unfold b_pg_g in H3.
+    rewrite H3 in e. inversion e. subst. inversion H4. subst. apply H6. rewrite graph_unfold. right. exists v, l, r. split.
+    split. unfold gamma, biEdge. destruct (@only_two_neighbours adr nat natEqDec (@bm_bi adr nat O natEqDec G)x) as [v1 [v2 ?]].
+    unfold b_pg_g in H3. rewrite H3 in e. inversion e. subst. auto. auto. auto.
+  Qed.
+
+  Lemma graph_graphs_eq_l:
+    forall G v x l r w, lookup G x v l r w ->
+                        (trinode x v l r ⊗ (graph l G ⊗ graph r G) = graph l G ⊗ graphs (x :: l :: r :: nil) G)%pred.
+  Proof.
+    intros. apply lookup_graph_unfold in H. rewrite <- ocon_assoc. unfold graphs. rewrite ocon_emp. do 2 rewrite <- ocon_assoc.
+    rewrite (ocon_comm (graph l G) (graph x G)). rewrite (ocon_assoc (graph x G) (graph l G) (graph l G)).
+    rewrite ocon_precise_elim. rewrite (ocon_assoc (graph x G) (graph l G) (graph r G)). rewrite H.
+    rewrite (ocon_assoc (trinode x v l r) (graph l G) (graph r G)).
+    rewrite (ocon_assoc (trinode x v l r) (graph l G ⊗ graph r G) (graph l G ⊗ graph r G)). rewrite ocon_precise_elim. auto.
+    apply precise_ocon; apply precise_graph. apply precise_graph.
+  Qed.
+
   Lemma lem_subgraphupdate_l : forall G v G1 x v1 l r, valid (imp (and (star (graph l G1) (mwand (graph l G) (union (ptto_node x v l r) (union (graph l G) (graph r G))))) (and (subset_reach G l G1) (and (eq_notreach G l G1) (and (lookup G x v l r) (lookup G1 x v1 l r))))) (union (ptto_node x v1 l r) (union (graph l G1) (graph r G1)))).
-  Proof. admit. Qed.
-  
+  Proof.
+    intros. intro w; hnf. unfold and, star, union, mwand, subset_reach, eq_notreach, ptto_node. intros.
+    destruct H as [? [? [? [? ?]]]].
+    assert (subset (reachable_through_set (b_pg_g G) (l :: nil)) (reachable_through_set (b_pg_g G1) (l :: nil))).
+    unfold reachable_through_set. intro n; intros. destruct H4 as [s [? ?]]; exists s. split; auto. apply in_inv in H4.
+    destruct H4. subst. apply H0; auto. inversion H4. clear H0.
+    generalize (subgraph_update_ewand G G1 (l :: nil) (l :: nil) (x :: l :: r :: nil) H4 H1). intro.
+    unfold graphs in H0 at 1 2 3 5. do 2 rewrite ocon_emp in H0. apply graph_graphs_eq_l in H2. rewrite H2 in H.
+    specialize (H0 w H).  apply graph_graphs_eq_l in H3. rewrite H3. auto.
+  Qed.
+
+  Lemma graph_graphs_eq_r:
+    forall G v x l r w, lookup G x v l r w ->
+                        (trinode x v l r ⊗ (graph l G ⊗ graph r G) = graph r G ⊗ graphs (x :: l :: r :: nil) G)%pred.
+  Proof.
+    intros. apply lookup_graph_unfold in H. rewrite <- ocon_assoc. unfold graphs. rewrite ocon_emp. do 2 rewrite <- ocon_assoc.
+    rewrite (ocon_comm (graph r G) (graph x G)). rewrite H. rewrite (ocon_assoc (trinode x v l r ⊗ graph l G)).
+    rewrite ocon_precise_elim. rewrite (ocon_assoc (trinode x v l r)) at 2.
+    rewrite (ocon_assoc (trinode x v l r ⊗ (graph l G ⊗ graph r G))).
+    rewrite (ocon_assoc (trinode x v l r) (graph l G ⊗ graph r G) (graph l G ⊗ graph r G)). rewrite ocon_precise_elim.
+    rewrite ocon_assoc. auto. apply precise_ocon; apply precise_graph. apply precise_graph.
+  Qed.
+
   Lemma lem_subgraphupdate_r : forall G v G1 x v1 l r, valid (imp (and (star (graph r G1) (mwand (graph r G) (union (ptto_node x v l r) (union (graph l G) (graph r G))))) (and (subset_reach G r G1) (and (eq_notreach G r G1) (and (lookup G x v l r) (lookup G1 x v1 l r))))) (union (ptto_node x v1 l r) (union (graph l G1) (graph r G1)))).
-  Proof. admit. Qed.
-  
+  Proof.
+    intros. intro w; hnf. unfold and, star, union, mwand, subset_reach, eq_notreach, ptto_node. intros.
+    destruct H as [? [? [? [? ?]]]].
+    assert (subset (reachable_through_set (b_pg_g G) (r :: nil)) (reachable_through_set (b_pg_g G1) (r :: nil))).
+    unfold reachable_through_set. intro n; intros. destruct H4 as [s [? ?]]; exists s. split; auto. apply in_inv in H4.
+    destruct H4. subst. apply H0; auto. inversion H4. clear H0.
+    generalize (subgraph_update_ewand G G1 (r :: nil) (r :: nil) (x :: l :: r :: nil) H4 H1). intro.
+    unfold graphs in H0 at 1 2 3 5. do 2 rewrite ocon_emp in H0. apply graph_graphs_eq_r in H2. rewrite H2 in H.
+    specialize (H0 w H).  apply graph_graphs_eq_r in H3. rewrite H3. auto.
+  Qed.
+
   Lemma lem_pttoupdate : forall v G x v1 l r G1, valid (imp (and (star (ptto_node x v1 l r) (mwand (ptto_node x v l r) (union (ptto_node x v l r) (union (graph l G) (graph r G))))) (and (lookup G x v l r) (update G x v1 l r G1))) (union (ptto_node x v1 l r) (union (graph l G1) (graph r G1)))).
-  Proof. admit. Qed.
-    
+  Proof.
+    intros. intro w; hnf. unfold and, star, union, mwand, subset_reach, eq_notreach, ptto_node. intros.
+    destruct H as [? [? ?]]. generalize (lookup_graph_unfold _ _ _ _ _ _ H0); intro. destruct H1 as [Hn [Hi ?]].
+    apply eq_sym in H1. rewrite ocon_assoc in H2. rewrite <- H2 in H. destruct H0 as [? [? [? [? ?]]]].
+    assert (@gamma adr nat natEqDec (@bm_bi adr nat O natEqDec G) x = (v, l, r)). unfold gamma, biEdge.
+    destruct (@only_two_neighbours adr nat natEqDec (@bm_bi adr nat O natEqDec G) x) as [t1 [t2 ?]]. unfold b_pg_g in H6.
+    rewrite H6 in e. inversion e; subst. auto. generalize (single_graph_node_update_2_ewand G x v l r v1 G1 Hn Hi H7 H1 w H).
+    intro. assert (lookup G1 x v1 l r w). subst. split; simpl. unfold change_node_label. destruct (@t_eq_dec adr natEqDec x x).
+    auto. exfalso; auto. unfold change_valid. do 3 (split;auto). unfold change_edge_func. destruct (@t_eq_dec adr natEqDec x x).
+    auto. exfalso; auto. apply lookup_graph_unfold in H9. rewrite <- ocon_assoc. rewrite <- H9. apply H8.
+  Qed.
+
 End GraphMark.
