make_ramify.sh
@@ -9,3 +9,5 @@ coqc heap_model.v
 # coqc dag.v
 # coqc covariant_graph.v
 coqc spatial_graph.v
+coqc hip_graphmark.v
+coqc hip_graphmark_proofs.v
